

T.C.
İSTANBUL ÜNİVERSİTESİ
MÜHENDİSLİK FAKÜLTESİ

Sınav Sonucu	
İmza	İmza

For God's sake, don't
forget to write your ID

Fakülte Numarası : _____
Adı ve Soyadı : _____ :-)
Yarıyıl : _____
Ders : _____
Bölümü : _____
Tarih : _____

1) $f(x) = \ln(x+1)(2x+1) = \ln(x+1) + \ln(2x+1)$. Let $u(x) = \ln(x+1)$. Repeated differentiation of $u(x) = \ln(x+1)$ yields

$$u'(x) = \frac{1}{x+1}, u''(x) = \frac{-1}{(x+1)^2}, u'''(x) = \frac{1 \cdot 2}{(x+1)^3}, u^{(4)}(x) = \frac{-1 \cdot 2 \cdot 3}{(x+1)^4} \dots u^{(n)} = \frac{(-1)^{n-1} (n-1)!}{(x+1)^n}$$

So we have $u^{(n)}(0) = (-1)^{n-1} (n-1)!$. Therefore the Maclaurin series of $u(x) = \ln(x+1)$ is

$$u(x) = \ln(x+1) = \sum_{n=0}^{\infty} \frac{(-1)^{n-1} (n-1)!}{n!} x^n = \sum_{n=0}^{\infty} \frac{(-1)^{n-1}}{n} x^n$$

If we replace x by $2x$ we get the following

$$u(2x) = \ln(2x+1) = \sum_{n=0}^{\infty} \frac{(-1)^{n-1}}{n} \frac{2^n x^n}{1}.$$

Then adding the above two series, we get

$$f(x) = \ln(x+1)(2x+1) = \ln(x+1) + \ln(2x+1) = u(x) + u(2x)$$

$$= \sum_{n=0}^{\infty} \frac{(-1)^{n-1}}{n} x^n + \sum_{n=0}^{\infty} \frac{(-1)^{n-1}}{n} \frac{2^n x^n}{1} = \sum_{n=0}^{\infty} \frac{(-1)^{n-1}}{n} (1+2^n) x^n.$$